Weidenbach_Book/IsaSAT_Setup.thy
@@ -553,51 +553,42 @@ lemma count_decided_st_alt_def: \<open>count_decided_st S = count_decided (get_t
 definition (in -) is_in_conflict_st :: \<open>nat literal \<Rightarrow> nat twl_st_wl \<Rightarrow> bool\<close> where
   \<open>is_in_conflict_st L S \<longleftrightarrow> is_in_conflict L (get_conflict_wl S)\<close>
 
-definition atm_is_in_conflict_st_heur :: \<open>nat literal \<Rightarrow> twl_st_wl_heur \<Rightarrow> bool\<close> where
-  \<open>atm_is_in_conflict_st_heur L = (\<lambda>(M, N, (_, D), _). atm_in_conflict_lookup (atm_of L) D)\<close>
+definition atm_is_in_conflict_st_heur :: \<open>nat literal \<Rightarrow> twl_st_wl_heur \<Rightarrow> bool nres\<close> where
+  \<open>atm_is_in_conflict_st_heur L = (\<lambda>(M, N, (_, D), _). do {
+     ASSERT (atm_in_conflict_lookup_pre (atm_of L) D); RETURN (\<not>atm_in_conflict_lookup (atm_of L) D) })\<close>
 
 lemma atm_is_in_conflict_st_heur_alt_def:
-  \<open>RETURN oo atm_is_in_conflict_st_heur = (\<lambda>L (M, N, (_, (_, D)), _). RETURN (D ! (atm_of L) \<noteq> None))\<close>
-  unfolding atm_is_in_conflict_st_heur_def by (auto intro!: ext simp: atm_in_conflict_lookup_def)
+  \<open>atm_is_in_conflict_st_heur = (\<lambda>L (M, N, (_, (_, D)), _). do {ASSERT ((atm_of L) < length D); RETURN (D ! (atm_of L) = None)})\<close>
+  unfolding atm_is_in_conflict_st_heur_def by (auto intro!: ext simp: atm_in_conflict_lookup_def atm_in_conflict_lookup_pre_def)
+
+lemma atm_of_in_atms_of_iff: \<open>atm_of x \<in> atms_of D \<longleftrightarrow> x \<in># D \<or> -x \<in># D\<close>
+  by (cases x) (auto simp: atms_of_def dest!: multi_member_split)
 
 lemma atm_is_in_conflict_st_heur_is_in_conflict_st:
-  \<open>(uncurry (RETURN oo atm_is_in_conflict_st_heur), uncurry (RETURN oo is_in_conflict_st)) \<in>
-   [\<lambda>(L, S). -L \<notin># the (get_conflict_wl S) \<and> get_conflict_wl S \<noteq> None \<and>
-     L \<in># \<L>\<^sub>a\<^sub>l\<^sub>l (all_atms_st S)]\<^sub>f
+  \<open>(uncurry (atm_is_in_conflict_st_heur), uncurry (mop_lit_notin_conflict_wl)) \<in>
+   [\<lambda>(L, S). True]\<^sub>f
    Id \<times>\<^sub>r twl_st_heur \<rightarrow> \<langle>Id\<rangle> nres_rel\<close>
 proof -
   have 1: \<open>aaa \<in># \<L>\<^sub>a\<^sub>l\<^sub>l A \<Longrightarrow> atm_of aaa  \<in> atms_of (\<L>\<^sub>a\<^sub>l\<^sub>l A)\<close> for aaa A
     by (auto simp: atms_of_def)
   show ?thesis
   unfolding atm_is_in_conflict_st_heur_def twl_st_heur_def option_lookup_clause_rel_def uncurry_def comp_def
+    mop_lit_notin_conflict_wl_def
   apply (intro frefI nres_relI)
   apply refine_rcg
   apply clarsimp
-  apply (subst atm_in_conflict_lookup_atm_in_conflict[THEN fref_to_Down_unRET_uncurry_Id])
-  unfolding prod.simps prod_rel_iff
-    apply (rule 1; assumption)
-   apply (auto; fail)
-  by (auto simp: is_in_conflict_st_def atm_in_conflict_def atms_of_def atm_of_eq_atm_of)
-qed
-
-lemma atm_is_in_conflict_st_heur_is_in_conflict_st_ana:
-  \<open>(uncurry (RETURN oo atm_is_in_conflict_st_heur), uncurry (RETURN oo is_in_conflict_st)) \<in>
-   [\<lambda>(L, S). -L \<notin># the (get_conflict_wl S) \<and> get_conflict_wl S \<noteq> None \<and>
-     L \<in># \<L>\<^sub>a\<^sub>l\<^sub>l (all_atms_st S)]\<^sub>f
-   Id \<times>\<^sub>r twl_st_heur_conflict_ana  \<rightarrow> \<langle>Id\<rangle> nres_rel\<close>
-proof -
-  have 1: \<open>aaa \<in># \<L>\<^sub>a\<^sub>l\<^sub>l A \<Longrightarrow> atm_of aaa  \<in> atms_of (\<L>\<^sub>a\<^sub>l\<^sub>l A)\<close> for aaa A
-    by (auto simp: atms_of_def)
-  show ?thesis
-  unfolding atm_is_in_conflict_st_heur_def twl_st_heur_conflict_ana_def option_lookup_clause_rel_def
-  apply (intro frefI nres_relI)
-  apply (case_tac x, case_tac y)
-  apply clarsimp
-  apply (subst atm_in_conflict_lookup_atm_in_conflict[THEN fref_to_Down_unRET_uncurry_Id])
-  unfolding prod.simps prod_rel_iff
-    apply (rule 1; assumption)
-   apply (auto; fail)
-  by (auto simp: is_in_conflict_st_def atm_in_conflict_def atms_of_def atm_of_eq_atm_of)
+  subgoal
+     apply (rule atm_in_conflict_lookup_pre)
+     unfolding \<L>\<^sub>a\<^sub>l\<^sub>l_all_atms_all_lits[symmetric]
+     apply assumption+
+     done
+  subgoal for x y x1 x2 x1a x2a x1b x2b x1c x2c x1d x1e x2d x2e
+    apply (subst atm_in_conflict_lookup_atm_in_conflict[THEN fref_to_Down_unRET_uncurry_Id, of \<open>all_atms_st x2\<close>  \<open>atm_of x1\<close> \<open>the (get_conflict_wl (snd y))\<close>])
+    apply (simp add: \<L>\<^sub>a\<^sub>l\<^sub>l_all_atms_all_lits atms_of_def)[]
+    apply (auto simp add: \<L>\<^sub>a\<^sub>l\<^sub>l_all_atms_all_lits atms_of_def option_lookup_clause_rel_def)[]
+    apply (simp add: atm_in_conflict_def atm_of_in_atms_of_iff)
+    done
+  done
 qed
 
 
